$9. ~~~ 1^{\circ}$ Растави на чиниоце
<br>
$~~~~~~~~~~~~~$ i) $2x^2+x-15;$
<br>
$~~~~~~~~~~~~$ ii) $3x^2-8x+4.$
<br>
$~~~~~~ 2^{\circ}$ Скртатити разломке:
<br>
$~~~~~~~~~~~~~$ i) $\displaystyle \frac{2x^2-7x+3}{2x^2-9x+4}$
<br>

$~~~~~~~~~~~~$ ii) $\displaystyle \frac{4x^2-19x+12}{12x^2-x-6}$

Resenje:

$1^{\circ}$

$i)$

$2x^2 +x - 15, a = 2, b = 1, c = -15$

$x_{1/2} = \displaystyle \frac{-b \pm \sqrt{-b^2 - 4ac}}{2a}$

$x_{1/2} = \displaystyle \frac{-1 \pm \sqrt{-1^2 - 4 \cdot 2 \cdot (-15)}}{2 \cdot 2}$

$x_{1/2} = \displaystyle \frac{-1 \pm \sqrt{(-1)^2 - 4 \cdot 2 \cdot (-15)}}{2 \cdot 2}$

$x_{1/2} = \displaystyle \frac{-1 \pm \sqrt{121}}{4}$

$x_{1/2} = \displaystyle \frac{-1 \pm 11}{4}$

$x_1 = \displaystyle \frac{5}{2}, x_2 = -3$

$a(x - x_1)(x - x_2) = 2(x - \displaystyle \frac{5}{2})(x + 3)$

$ii)$

$3x^2 - 8x + 4, a = 3, b = -8, c = 4$

$x_{1/2} = \displaystyle \frac{-b \pm \sqrt{-b^2 - 4ac}}{2a}$

$x_{1/2} = \displaystyle \frac{8 \pm \sqrt{64 - 48}}{6}$

$x_{1/2} = \displaystyle \frac{8 \pm 4}{6}$

$x_1 = \displaystyle \frac{2}{3}, x_2 = 2$

$a(x - x_1)(x - x_2) = 3(x - \displaystyle \frac{2}{3})(x - 2)$

$2^{\circ}$

$i)$

$\displaystyle \frac{2x^2-7x+3}{2x^2-9x+4}$

$2x^2-7x+3, a = 2, b = -7, c = 3$

$x_{1/2} = \displaystyle \frac{7 \pm \sqrt{49 - 24}}{4}$

$x_{1/2} = \displaystyle \frac{7 \pm 5}{4}$

$x_1 = 1/2, x_2 = 3$

$2(x - 1/2)(x - 3)$

$2x^2-9x+4, a = 2, b = -9, c =4$

$x_{1/2} = \displaystyle \frac{-b \pm \sqrt{-b^2 - 4ac}}{2a}$

$x_{1/2} = \displaystyle \frac{9 \pm \sqrt{81 - 32}}{4}$

$x_{1/2} = \displaystyle \frac{9 \pm 7}{4}$

$x_1 = 4, x_2 = 1/2$

$2(x-4)(x-1/2)$

$\displaystyle \frac{2(x - 1/2)(x - 3)}{2(x-4)(x-1/2)}$

$\displaystyle \frac{\cancel 2 \cancel{(x - 1/2)}(x - 3)}{\cancel 2(x-4)\cancel{(x-1/2)}}$

$\displaystyle \frac{x-3}{x-4}$

$ii)$

$\displaystyle \frac{4x^2-19x+12}{12x^2-x-6}$

$4x^2-19x+12, a = 4, b = -19, c = 12$

$x_{1/2} = \displaystyle \frac{-b \pm \sqrt{-b^2 - 4ac}}{2a}$

$x_{1/2} = \displaystyle \frac{19 \pm \sqrt{361 - 192}}{8}$

$x_{1/2} = \displaystyle \frac{19 \pm 13}{8}$

$x_1 = 4, x_2 = 3/4$

$4(x - 4)(x - 3/4)$

$12x^2-x-6, a = 12, b = -1, c = -6$

$x_{1/2} = \displaystyle \frac{-b \pm \sqrt{-b^2 - 4ac}}{2a}$

$x_{1/2} = \displaystyle \frac{1 \pm \sqrt{1 +288}}{24}$

$x_{1/2} = \displaystyle \frac{1 \pm 17}{24}$

$x_1 = 3/4, x_2 = -2/3$

$12(x - 3/4)(x + 2/3)$

$\displaystyle \frac{4(x - 4)(x - 3/4)}{12(x - 3/4)(x + 2/3)}$

$\displaystyle \frac{ 4(x - 4)(x - 3/4)}{12(x - 3/4)(x + 2/3)}$

$\displaystyle \frac{\cancel 4(x - 4)\cancel{(x - 3/4)}}{\cancel 12 \cancel{(x - 3/4)}(x + 2/3)}$














