11. Решити једначине

$\displaystyle 1^{\circ} \frac{2x+1}{x^2+x-6} - \frac{x-1}{x^2-5x+6} = \frac{6}{x^2-9}$

$\displaystyle 2^{\circ} \frac{1}{x^2 - 3x - 10} - \frac{1}{x^2 + 7x + 10} =   \frac{1}{x^2-4} - \frac{1}{x^2 - 7x + 10}$

$\displaystyle 3^{\circ} \frac{2x^2 - 10x + 9}{x^2 - 4x - 12} = \frac{x^2 - x - 9}{(x-6)(x+2)}$

Решења:

$\displaystyle 1^{\circ} \frac{2x+1}{x^2+x-6} - \frac{x-1}{x^2-5x+6} = \frac{6}{x^2-9}$

$\displaystyle \frac{2x+1}{x^2+x-6} - \frac{x-1}{x^2-5x+6} = \frac{6}{(x-3)*(x+3)}$

$\displaystyle 3^{\circ} \frac{2x^2 - 10x + 9}{x^2 - 4x - 12} = \frac{x^2 - x - 9}{(x-6)(x+2)}$

$\displaystyle \frac{2x^2 - 10x + 9}{(x-6)(x+2)} = \frac{x^2 - x - 9}{(x-6)(x+2)}$

Ако $x$ није $6$ или $-2$ важи:

$\displaystyle 2x^2 - 10x + 9 = x^2 - x - 9$

$\displaystyle x^2 - 9x + 18 = 0$

$\displaystyle x_{1,2} = $