11. Израз $(x^2 + y^2 + z^2 + xy + yz + zx)^2 - (x + y + z)^2(x^2 + y^2 + z^2)$ идентички је једнак::

    $(А)$ $(x + y + z) ^ 4$
    
    $(B)$ $(xy + yz + zx)^2$

    $(C)$ $x^2y^2 + y^2z^2 + z^2x^2$

    $(D)$ $3xyz(x + y + z)$

    $(E)$ $(x + y + z)^2(xy + yz + zx)$

Решење.


$(x^2 + y^2 + z^2) = a$

$(xy + yz + zx) = b$

$(x^2 + y^2 + z^2 + xy + yz + zx)^2 - (x + y + z)^2(x^2 + y^2 + z^2) =$ 

$((x^2 + y^2 + z^2) + (xy + yz + zx))^2 - (x^2 + y^2 + z^2 + 2xy + 2yz + 2zx)(x^2 + y^2 + z^2) =$

$((x^2 + y^2 + z^2) + (xy + yz + zx))^2 - ((x^2 + y^2 + z^2) + 2(xy + yz + zx))(x^2 + y^2 + z^2) =$

$(a + b)^2 - (a + 2b)a  =$

$ a^2 + 2ab + b^2 - (a^2 + 2ab)  =$

$ a^2 + 2ab + b^2 - a^2 - 2ab  =$

$ b^2 = (xy + yz + zx)^2$




