$34.$ Упростити израз
$$E = \displaystyle \sqrt{\frac{x+3a}{4a} + \sqrt{\frac{x-a}{a}}}+\sqrt{\frac{x+3a}{4a} +-\sqrt{\frac{x-a}{a}}}, ~~~~a > 0. $$

$Решење.$ Израз $E (E > 0)$ је дефинисан за $x \ge a$. Прва поткорена величина је очигледно позитивна, док је друга

$$\displaystyle \frac{x+3a}{4a} - \sqrt{\frac{x-a}{a}} \ge 0 \equiv (x - 5a)^2 \ge 0. $$
Сада имамо
$$E^2 = 2 \displaystyle \frac{x+3a}{4a} + 2 \sqrt{(\frac{x+3a}{4a})^2 - \frac{x-a}{a}}$$
$$= \displaystyle \frac{x+3a}{2a} + 2\sqrt{(\frac{x-5a}{4a})^2} = \frac{x+3a}{2a} + 2\Bigl|\frac{x-5a}{4a}\Bigr|$$
$$= \displaystyle \frac{x + 3a}{2a} + \frac{|x-5a}{2a}, јер ~ је ~ a > 0.$$
Ако је

$i) ~ a \le x < 5a,$ тада је $E^2 = \displaystyle \frac{x+3a}{2a} + \frac{-(x-5a)}{2a} = 4 \to E= 2;$

$ii)~ 5a \le x$, тада је $E^2 = \displaystyle \frac{x+3a}{2a} + \frac{x-5a}{2a} = \frac{x - a}{a} \to E= \sqrt{\frac{x-a}{a}}.$

Дакле,

