18. Користећи биномну формулу израчунати:

$1. \ (2-x)^6$

$2. \ (a^3-b)^5$

Решење:

$$ (x+y)^n =\binom{n}{0}x^ny^0+\binom{n}{1}x^{n-1}y^1+\binom{n}{2}x^{n-2}y^2+\dots+\binom{n}{k}x^{n-k}y^k+\dots+\binom{n}{n}x^0y^n= \sum_{k=0}^{n} \binom{n}{k}x^{n-k}y^k$$

$$ (x+y)^6 =\binom{6}{0}x^6y^0+\binom{6}{1}x^{5}y^1+\binom{6}{2}x^{4}y^2+\dots+\binom{6}{k}x^{6-k}y^k+\dots+\binom{6}{6}x^0y^6= \sum_{k=0}^{6} \binom{6}{k}x^{6-k}y^k$$

$$ \binom{6}{0}=\binom{6}{6}=1$$

$$ \binom{6}{1}=\binom{6}{5}=6$$

$$ \binom{6}{2}=\binom{6}{4}=\frac{6\cdot5}{2\cdot1}=15$$

$$ \binom{6}{3}=\frac{6\cdot5\cdot4}{3\cdot2\cdot1}=20$$

$1. \ (2-x)^6=$<br>
$\binom{6}{0}2^6(-x)^0+\binom{6}{1}2^{5}(-x)^1+\binom{6}{2}2^{4}(-x)^2+\binom{6}{3}2^{3}(-x)^3+\binom{6}{4}2^{2}(-x)^4+\binom{6}{5}2^{1}(-x)^5+\binom{6}{6}2^0(-x)^6=$<br>
$1\cdot2^6-6\cdot2^5x+15\cdot2^4\cdot x^2-20\cdot2^3\cdot x^3+15\cdot2^2\cdot x^4-6\cdot2^1\cdot x^5+1\cdot2^0\cdot x^6=$<br>
$1\cdot64-6\cdot32x+15\cdot16\cdot x^2-20\cdot8\cdot x^3+15\cdot4\cdot x^4-6\cdot2\cdot x^5+1\cdot1\cdot x^6=$<br>
$64-192x+240x^2-160x^3+60x^4-12x^5+x^6$

$2. \ (a^3-b)^5=$<br>
$\binom{5}{0}(a^3)^5(-b)^0+\binom{5}{1}(a^3)^{4}(-b)^1+\binom{5}{2}(a^3)^{3}(-b)^2+\binom{5}{3}(a^3)^{2}(-b)^3+\binom{5}{4}(a^3)^{1}(-b)^4+\binom{5}{5}(a^3)^{0}(-b)^5=$<br>
$1a^{15}(-b)^0+5a^{12}(-b)^1+10a^{9}(-b)^2+10a^{6}(-b)^3+5a^{3}(-b)^4+1a^{0}(-b)^5=$<br>
$a^{15}-5a^{12}b+10a^{9}b^2-10a^{6}b^3+5a^{3}b^4-b^5$
